Blog/Posts/FloatQanda.lean
@@ -1,19 +1,25 @@
----
-title: "Floats in Lean 4.33"
-date: 2026-06-19T09:00:00+02:00
-categories:
-  - blog
-tags:
-  - Lean
-  - Floating-point numbers
----
+import VersoBlog
+import Blog.Tags
+
+open Verso Genre Blog
+open Blog.Tag
+
+set_option pp.rawOnError true
+
+#doc (Post) "Floats in Lean 4.33" =>
+
+%%%
+authors := ["Julia Markus Himmel"]
+date := {year := 2026, month := 6, day := 19}
+categories := [lean, floats]
+%%%
 
 Here is a little informal Q&A-style post about the changes to `Float` in Lean
 4.33. The questions are meant to be read from top to bottom, not in arbitrary
 order. This is not an "official" communication by the Lean FRO, whatever that
 may mean.
 
-## What is changing about floats in Lean 4.33?
+# What is changing about floats in Lean 4.33?
 
 Up until Lean 4.32, the `Float` type and all operations defined on it were
 opaque to Lean's kernel. This means that it was possible to write programs
@@ -21,7 +27,7 @@ involving floats, and the compiler would happily compile them directly to C's
 `double` type, but it was not possible to prove anything about the float
 operations.
 
-Starting in Lean 4.33, `Float`, and *some* of the functions defined for floats,
+Starting in Lean 4.33, `Float`, and _some_ of the functions defined for floats,
 now have a definition. `Float` is now (after
 [#14091](https://github.com/leanprover/lean4/pull/14091)) a wrapper around a
 new type `Float.Model` (which was added in
@@ -50,7 +56,7 @@ instead of using your CPU's native floating-point support. This way, you can
 achieve a spectacular 200x speed-down on your code with the added bonus of far
 fewer supported operations and an overall suboptimal experience.
 
-## How can I use this?
+# How can I use this?
 
 The boring use case is that floating-point operations now execute in the
 kernel, so that you can prove `0.1 + 0.2 != 0.3` with `rfl`. However, you should
@@ -62,23 +68,24 @@ The other, much more interesting, use case is that it is now, in principle,
 possible to prove all kinds of properties about Lean programs involving the
 `Float` type. This brings us to the important bit.
 
-## The important bit
+# The important bit
 
 The `Float.Model` type and its associated theory are
-**not** a fully-featured general-purpose floating-point library, and they will
+*not* a fully-featured general-purpose floating-point library, and they will
 never be one. Neither we, nor anyone else, should develop extensive theory
 about the `Float.Model` type and prove lemmas directly about this type.
 
 Instead, if you are interested in proving things about your programs involving
 `Float`, here is what you should do:
-- In a downstream library, develop a fully-featured general-purpose
+
+* In a downstream library, develop a fully-featured general-purpose
   floating-point library, for example by porting Flocq, or by porting SymFPU,
-  or by reading the IEEE-754 specification (and maybe the *Handbook of
-  Floating-Point Arithmetic*) and writing something from scratch
-- Prove that the `Float.Model` type is equivalent to your type corresponding to
+  or by reading the IEEE-754 specification (and maybe the _Handbook of
+  Floating-Point Arithmetic_) and writing something from scratch
+* Prove that the `Float.Model` type is equivalent to your type corresponding to
   the IEEE binary64 format without NaN payloads, and that all of the operations
   commute with that equivalence
-- Transfer lemmas about your nice downstream float type to `Float.Model` along
+* Transfer lemmas about your nice downstream float type to `Float.Model` along
   that equivalence
 
 Doing the verification layers separately like this is a good idea because the
@@ -94,27 +101,27 @@ if we planned to add a floating-point verification layer to the Lean standard
 library, which we are not planning to do, we would make this entirely separate
 from the construction of `Float.Model`.
 
-## Are you going to ship lemmas about `Float` as part of the Lean distribution?
+# Are you going to ship lemmas about `Float` as part of the Lean distribution?
 
 No, see above.
 
-## Are you adding a general-purpose floating-point library to the Lean standard library?
+# Are you adding a general-purpose floating-point library to the Lean standard library?
 
 No, see above. Note also that it would be quite difficult for us to do this,
 because we don't have plans to add a real number type to the Lean distribution,
 which is a prerequisite for a proper float verification layer.
 
-## I am writing a pure proof development involving floating-point numbers and I have no plans to execute my code. Is the new material useful to me?
+# I am writing a pure proof development involving floating-point numbers and I have no plans to execute my code. Is the new material useful to me?
 
 No.
 
-## I have goals about `Float` or `Float32` that I want to bitblast and dispatch using `bv_decide`. Can I do this now?
+# I have goals about `Float` or `Float32` that I want to bitblast and dispatch using `bv_decide`. Can I do this now?
 
 Our model is not set up to allow this. However, you can connect `Float.Model`
 to a library like [fp-lean](https://github.com/opencompl/fp-lean), transfer your
 statement over to their bitblastable floats and then bitblast that.
 
-## How was the model constructed?
+# How was the model constructed?
 
 While it is not a direct port, part of the code of the model we use
 (specifically the `UnpackedFloat` type and the rounding logic) is quite
@@ -124,15 +131,15 @@ of additional operations and also a packing/unpacking layer (Flocq probably also
 has this, but our packing/unpacking code was developed independently). There are
 several good reasons to stay true to the prior art here:
 
-- Flocq is an excellent piece of software, and there is no reason to reinvent
+* Flocq is an excellent piece of software, and there is no reason to reinvent
   the wheel.
-- Flocq has had many eyes on it, so by staying close to it we are increasing
+* Flocq has had many eyes on it, so by staying close to it we are increasing
   the likelihood that our model is correct.
-- Realistically, it is very likely that whatever turns out to be the dominant
+* Realistically, it is very likely that whatever turns out to be the dominant
   Lean library for floats will be derived from Flocq. If our model is also
   derived from Flocq, then proving the two approaches equivalent should be an
   easier task.
-- Since we are all bound by the IEEE specification, all implementations will be
+* Since we are all bound by the IEEE specification, all implementations will be
   somewhat similar anyways.
 
 It is safe to say that our model would not be as good if not for Flocq. I tried
@@ -143,17 +150,17 @@ arithmetic and the rounding procedure in particular easier to learn.
 Besides the implementation, various other resources were useful to me,
 including:
 
-- A blog post titled [Floating Point Numbers and
+* A blog post titled [Floating Point Numbers and
   Rounding](https://drilian.com/posts/2023.01.10-floating-point-numbers-and-rounding/)
   (though be aware that there are some typos in the calculations)
-- The *Handbook of Floating-Point Arithmetic*.
+* The _Handbook of Floating-Point Arithmetic_.
 
-## Where can I look at the model?
+# Where can I look at the model?
 
 [Here](https://github.com/leanprover/lean4/blob/bc5f89f4abe82ee105ce7922a83e286fd7a67774/src/Init/Data/Float/Model/Float.lean)
 is a link to the code.
 
-## Is the model correct?
+# Is the model correct?
 
 This question is more subtle than it may seem, because we first have to define
 what it means to be "correct". The central goal of `Float.Model` is to behave
@@ -165,13 +172,13 @@ So, how do the runtime float
 functions behave when executed? Since Lean compiles to C, we are effectively
 governed by the C standard here. In typical C fashion, the semantics of
 floating-point operations are a minefield of undefined behavior and
-implementation-defined behavior. There is an article called [*The pitfalls of
-verifying floating-point operations*](https://arxiv.org/pdf/cs/0701192) which
+implementation-defined behavior. There is an article called [_The pitfalls of
+verifying floating-point operations_](https://arxiv.org/pdf/cs/0701192) which
 discusses many potential problems. For Lean, the short version is this: we
 hardened the runtime a bit ([1](https://github.com/leanprover/lean4/pull/13872)
 [2](https://github.com/leanprover/lean4/pull/13930)
-[3](https://github.com/leanprover/lean4/pull/14012)), and now, *as long as code
-called via FFI does not mess with the floating-point environment*, we can be
+[3](https://github.com/leanprover/lean4/pull/14012)), and now, _as long as code
+called via FFI does not mess with the floating-point environment_, we can be
 confident to observe the behavior required by IEEE 754. The conversions
 between floats and integers are an exception, because for these the C standard
 has its own opinion about
@@ -212,18 +219,18 @@ the decimal-to-float routine.
 As time progresses, hopefully people will show our model equivalent to their
 models, which should further increase confidence.
 
-## Which operations are supported?
+# Which operations are supported?
 
 As of writing: `add`, `sub`, `mul`, `div`, `sqrt`, `abs`, `neg`, `isNaN`,
 `isInf`, `isFinite`, `le`, `lt`, `beq`, `ofInt`, `ofNat`, `ofIntX`, `ofUIntX`,
 `toIntX`, `toUIntX`, `ofScientific`.
 
-## Are you going to support more operations?
+# Are you going to support more operations?
 
 Yes, there are some more that we hope to get to in the short term (before the
 release of 4.33 perhaps), such as `ceil`, `floor`, `round` and `scaleB`.
 
-## Will you add my favorite operation?
+# Will you add my favorite operation?
 
 It depends. As so often it is a question of how expensive it would be to add,
 and how useful having it would be.
@@ -252,11 +259,11 @@ and/or open an RFC. As with all feature suggestions to Lean, the ones that are
 most likely to get acted on are those which unlock a relevant and real use case
 instead of just being something that would be cool to have.
 
-## Will you consider my pull request adding a model for a new operation?
+# Will you consider my pull request adding a model for a new operation?
 
 No.
 
-## Why not?
+# Why not?
 
 With all of the considerations described above and the fact that getting this
 wrong is a miscompilation, reviewing a PR adding a new model is more expensive
