examples/mvcgen/Mvcgen.lean
@@ -1,0 +1,132 @@
+/-
+Code for the blog post "My first verified (imperative) program" (2025-07-06).
+
+This is the code from
+https://gist.github.com/TwoFX/bcdb6202fa8d8024b6a766a4d9df3f30
+which accompanies the post. It uses the *old* `mvcgen` syntax from the
+Lean 4.22 preview of `Std.Do`, as described in the post.
+-/
+import Std.Data.HashSet.Lemmas
+import Std.Tactic.Do
+
+open Std Do
+
+/-!
+# Missing standard library material that will be part of a future Lean release
+-/
+
+namespace List
+
+theorem exists_mem_iff_exists_getElem (P : α → Prop) (l : List α) :
+    (∃ x ∈ l, P x) ↔ ∃ (i : Nat), ∃ hi, P (l[i]'hi) := by
+  grind [mem_iff_getElem]
+
+/--
+`l.ExistsPair P` asserts that there are indices `i` and `j` such that `i < j` and `P l[i] l[j]` is true.
+-/
+structure ExistsPair (P : α → α → Prop) (l : List α) where
+  not_pairwise : ¬l.Pairwise (¬P · ·)
+
+theorem existsPair_iff_not_pairwise {P : α → α → Prop} {l : List α} :
+    l.ExistsPair P ↔ ¬l.Pairwise (fun x y => ¬P x y) := by
+  grind [ExistsPair]
+
+@[simp, grind]
+theorem not_existsPair_nil {P : α → α → Prop} : ¬[].ExistsPair P := by
+  simp [existsPair_iff_not_pairwise]
+
+@[simp, grind]
+theorem existsPair_cons {P : α → α → Prop} {x : α} {xs : List α} :
+    (x::xs).ExistsPair P  ↔ (∃ y ∈ xs, P x y) ∨ xs.ExistsPair P := by
+  grind [List.existsPair_iff_not_pairwise]
+
+@[simp, grind]
+theorem existsPair_append {P : α → α → Prop} {xs ys : List α} :
+    (xs ++ ys).ExistsPair P ↔ xs.ExistsPair P ∨ ys.ExistsPair P ∨ (∃ x ∈ xs, ∃ y ∈ ys, P x y) := by
+  grind [List.existsPair_iff_not_pairwise]
+
+@[simp]
+theorem Zipper.pref_mk {l : List α} {rpref suff h} :
+    (List.Zipper.mk rpref suff h : List.Zipper l).pref = rpref.reverse := rfl
+
+end List
+
+-- Tell Lean that it doesn't need to warn us that `mvcgen` is still a pre-release.
+set_option mvcgen.warning false
+
+-- ANCHOR: full
+/-!
+# Imperative implementation
+-/
+
+-- ANCHOR: impl
+def pairsSumToZero (l : List Int) : Id Bool := do
+  let mut seen : HashSet Int := ∅
+
+  for x in l do
+    if -x ∈ seen then
+      return true
+    seen := seen.insert x
+
+  return false
+-- ANCHOR_END: impl
+
+/-!
+# Verification of imperative implementation
+-/
+
+-- ANCHOR: spec
+theorem pairsSumToZero_spec (l : List Int) :
+    ⦃⌜True⌝⦄ pairsSumToZero l ⦃⇓r => r = true ↔ l.ExistsPair (fun a b => a + b = 0)⦄
+-- ANCHOR_END: spec
+    := by
+-- ANCHOR: vcgen
+  mvcgen [pairsSumToZero]
+-- ANCHOR_END: vcgen
+
+-- ANCHOR: inv
+  case inv =>
+    exact (fun (⟨earlyReturn?, seen⟩, traversalState) =>
+      (earlyReturn? = none ∧ (∀ x, x ∈ seen ↔ x ∈ traversalState.rpref) ∧ ¬traversalState.pref.ExistsPair (fun a b => a + b = 0)) ∨
+      (earlyReturn? = some true ∧ l.ExistsPair (fun a b => a + b = 0) ∧ l = traversalState.pref), ())
+-- ANCHOR_END: inv
+
+-- ANCHOR: allGoals
+  all_goals simp_all <;> grind
+-- ANCHOR_END: allGoals
+-- ANCHOR_END: full
+
+namespace Functional
+
+/-!
+# Bonus: functional implementation
+-/
+
+-- ANCHOR: funImpl
+def pairsSumToZero (l : List Int) : Bool :=
+  go l ∅
+where
+  go (m : List Int) (seen : HashSet Int) : Bool :=
+    match m with
+    | [] => false
+    | x::xs => if -x ∈ seen then true else go xs (seen.insert x)
+-- ANCHOR_END: funImpl
+
+/-!
+# Bonus: verification of functional implementation
+-/
+
+-- ANCHOR: funGoSpec
+theorem pairsSumToZero_go_iff (l : List Int) (seen : HashSet Int) :
+    pairsSumToZero.go l seen = true ↔
+      l.ExistsPair (fun a b => a + b = 0) ∨ ∃ a ∈ seen, ∃ b ∈ l, a + b = 0 := by
+  fun_induction pairsSumToZero.go <;> simp_all <;> grind
+-- ANCHOR_END: funGoSpec
+
+-- ANCHOR: funFinal
+theorem pairsSumToZero_iff (l : List Int) :
+    pairsSumToZero l = true ↔ l.ExistsPair (fun a b => a + b = 0) := by
+  simp [pairsSumToZero, pairsSumToZero_go_iff]
+-- ANCHOR_END: funFinal
+
+end Functional
